Fix proof; some more boilerplate

src/program_proof/tutorial/lockservice/proof.v
@@ -1,7 +1,6 @@
 From Perennial.program_proof Require Import grove_prelude.
 From Goose.github_com.mit_pdos.gokv.tutorial Require Import lockservice.
-
-(* This is boilerplate. *)
+From Perennial.program_proof.grove_shared Require Import urpc_proof.
 
 Section marshal_proof.
 Context `{!heapGS Σ}.
@@ -43,3 +42,131 @@ Proof.
 Admitted.
 
 End marshal_proof.
+
+Section rpc_definitions.
+(* NOTE: "global" context because RPC specs are known by multiple machines. *)
+Context `{!gooseGlobalGS Σ}.
+Definition tryAcquire_core_spec (args:u64) (Φ:u64 → iPropO Σ): iPropO Σ.
+Admitted.
+
+Definition release_core_spec (args:u64) (Φ:iPropO Σ): iPropO Σ.
+Admitted.
+
+Definition getFreshNum_core_spec (Φ:u64 → iPropO Σ): iPropO Σ.
+Admitted.
+
+End rpc_definitions.
+
+Section encoded_rpc_definitions.
+(* This section is boilerplate. *)
+Context `{!gooseGlobalGS Σ}.
+Context `{!urpcregG Σ}.
+
+Program Definition getFreshNum_spec :=
+  λ (enc_args:list u8), λne (Φ : list u8 -d> iPropO Σ) ,
+  (
+  getFreshNum_core_spec (λ num, ∀ enc_reply, ⌜enc_reply = u64_le num⌝ -∗ Φ enc_reply)
+  )%I
+.
+Next Obligation.
+  (* solve_proper.
+Defined. *)
+Admitted.
+
+Program Definition tryAcquire_spec :=
+  λ (enc_args:list u8), λne (Φ : list u8 -d> iPropO Σ) ,
+  (∃ args,
+   ⌜enc_args = u64_le args⌝ ∗
+   tryAcquire_core_spec args (λ err, ∀ enc_reply, ⌜enc_reply = u64_le err⌝ -∗ Φ enc_reply)
+  )%I
+.
+Next Obligation.
+  (* solve_proper.
+Defined. *)
+Admitted.
+
+Program Definition release_spec :=
+  λ (enc_args:list u8), λne (Φ : list u8 -d> iPropO Σ) ,
+  (∃ args,
+   ⌜enc_args = u64_le args⌝ ∗
+   release_core_spec args (Φ [])
+  )%I
+.
+Next Obligation.
+  (* solve_proper.
+Defined. *)
+Admitted.
+
+Definition is_lockserver_host host : iProp Σ :=
+  ∃ γrpc,
+  "#H1" ∷ handler_spec γrpc host (U64 0) getFreshNum_spec ∗
+  "#H2" ∷ handler_spec γrpc host (U64 1) tryAcquire_spec ∗
+  "#H3" ∷ handler_spec γrpc host (U64 2) release_spec ∗
+  "#Hdom" ∷ handlers_dom γrpc {[ U64 0; U64 1; U64 2 ]}
+  .
+
+End encoded_rpc_definitions.
+
+Section start_server_proof.
+Context `{!heapGS Σ}.
+Context `{!urpcregG Σ}.
+
+Lemma wp_Server__Start s (host:u64) :
+  {{{
+        "#Hhost" ∷ is_lockserver_host host
+  }}}
+    Server__Start #s #host
+  {{{
+        RET #(); True
+  }}}
+.
+Proof.
+  iIntros (Φ) "Hpre HΦ".
+  iNamed "Hpre".
+  (* begin symbolic execution *)
+  wp_lam.
+  wp_pures.
+  wp_apply (map.wp_NewMap).
+  iIntros (handlers) "Hhandlers".
+
+  wp_pures.
+  wp_apply (map.wp_MapInsert with "Hhandlers").
+  iIntros "Hhandlers".
+  wp_pures.
+
+  wp_pures.
+  wp_apply (map.wp_MapInsert with "Hhandlers").
+  iIntros "Hhandlers".
+  wp_pures.
+
+  wp_pures.
+  wp_apply (map.wp_MapInsert with "Hhandlers").
+  iIntros "Hhandlers".
+  wp_pures.
+
+  wp_apply (urpc_proof.wp_MakeServer with "Hhandlers").
+  iIntros (r) "Hr".
+  wp_pures.
+
+  iNamed "Hhost".
+  wp_apply (wp_StartServer2 with "[$Hr]").
+  { set_solver. }
+  { (* Here, we show that the functions being passed in Go inside `handlers`
+       satisfy the spec they should. *)
+    (* First, show that the functions passed in are ALL the RPCs this host is
+       suppose to provide. *)
+    unfold handlers_complete.
+    repeat rewrite dom_insert_L.
+    rewrite dom_empty_L.
+    iSplitL "".
+    { iExactEq "Hdom". f_equal. set_solver. }
+
+    (* Now show the RPC specs, one at a time *)
+    iApply (big_sepM_insert_2 with "").
+    {
+      iExists _; iFrame "#".
+    }
+  }
+Qed.
+
+End start_server_proof.
